@prefix : <http://purl.org/nsoluti/oqs#>.
@prefix dc: <http://purl.org/dc/elements/1.1/> .
@prefix dcterms: <http://purl.org/dc/terms/> .
@prefix owl: <http://www.w3.org/2002/07/owl#> .
@prefix rdf: <http://www.w3.org/1999/02/22-rdf-syntax-ns#> .
@prefix xml: <http://www.w3.org/XML/1998/namespace> .
@prefix xsd: <http://www.w3.org/2001/XMLSchema#> .
@prefix foaf: <http://xmlns.com/foaf/0.1/> .
@prefix gufo: <http://purl.org/nemo/gufo#> .
@prefix rdfs: <http://www.w3.org/2000/01/rdf-schema#> .
@prefix time: <http://www.w3.org/2006/time#> .
@prefix vann: <http://purl.org/vocab/vann/> .
@prefix bibo: <http://purl.org/ontology/bibo/> .
@prefix opm: <http://openprovenance.org/model/opmo#> .
@prefix mod: <http://www.isibang.ac.in/ns/mod#> .
@prefix adms: <http://www.w3.org/ns/adms#> .
@prefix omv: <https://w3id.org/mod#> .
@prefix vs: <http://www.w3.org/2003/06/sw-vocab-status/ns#> .
@base <http://purl.org/nsoluti/oqs#> .

<http://purl.org/nsoluti/oqs#> rdf:type owl:Ontology ;
    owl:versionIRI <http://purl.org/nsoluti/oqs/1.0.0> ;
    owl:versionInfo "1.1.0"@en ;
    dc:creator "Marques, Yuri Bento" ,
               "Bax, Marcello Peixoto" ,
               "Pinheiro, Paulo" ;
    dc:title "OQS: Ontology for Questionnaires Sharing"@en ;
    dcterms:bibliographicCitation "Marques, Yuri Bento, Marcello Peixoto Bax, and Paulo Pinheiro. \"OQS: Ontology for Questionnaires Sharing.\", 2025, http://purl.org/nsoluti/doc/oqs ."@en ;
    dcterms:created "2025-01-15"^^xsd:date ;
    dcterms:modified "2025-01-15"^^xsd:date ;
    dcterms:license <http://creativecommons.org/licenses/by/4.0/legalcode> ;
    dcterms:issued "2025-01-15"^^xsd:date ;
    dcterms:publisher <https://nsoluti.ifnmg.edu.br> ;
    bibo:doi "10.5281/zenodo.XXXXXX" ;
    foaf:logo <https://nsoluti.github.io/oqs/logo.png> ;
    dcterms:source <https://github.com/nsoluti/oqs> ;
    omv:status "Stable"@en ;
    owl:versionInfo "1.1.0"@en ;
    owl:priorVersion <http://purl.org/nsoluti/oqs#/1.0.0> ;
    owl:backwardCompatibleWith <http://purl.org/nsoluti/oqs#/1.0.0> ;
    vann:preferredNamespacePrefix "oqs"@en ;
    vann:preferredNamespaceUri "https://purl.org/nsoluti/oqs#"^^xsd:anyURI ;
    vs:term_status "stable"@en ;
    rdfs:comment """  Cite this work as:     This work is distributed under Creative Commons Attribution License CC BY 4.0 <https://creativecommons.org/licenses/by/4.0/legalcode>.  For the source repository, see: <https://github.com/nsoluti/oqs>"""@en ;
    owl:imports gufo:.

:DataCollectionInstrument rdf:type owl:Class, gufo:Category, owl:NamedIndividual;
    rdfs:subClassOf gufo:FunctionalComplex;
    rdfs:label "DataCollectionInstrument"@en.
:Detector rdf:type owl:Class, gufo:Category, owl:NamedIndividual;
    rdfs:subClassOf gufo:FunctionalComplex;
    rdfs:label "Detector"@en.
:Person rdf:type owl:Class, gufo:Kind, owl:NamedIndividual;
    rdfs:subClassOf gufo:FunctionalComplex;
    rdfs:label "Person"@en.
:Questionnaire rdf:type owl:Class, gufo:Kind, owl:NamedIndividual;
    rdfs:label "Questionnaire"@en.
:QuestionnaireValidation rdf:type owl:Class, gufo:EventType, owl:NamedIndividual;
    rdfs:subClassOf gufo:Event;
    rdfs:label "QuestionnaireValidation"@en.
:QuestionnaireValidationType rdf:type owl:Class, gufo:AbstractIndividualType, owl:NamedIndividual;
    rdfs:subClassOf gufo:QualityValue;
    owl:equivalentClass [
  rdf:type owl:Class;
  owl:oneOf (:ContentValidation :SemanticValidation :PreTest :MathematicalValidation :ConstructValidity :CriterionValidity :FaceValidity :ReliabilityTesting :CulturalValidation :OtherValidation)
].
:ContentValidation rdf:type :QuestionnaireValidationType;
    rdf:label "[object Object]".
:SemanticValidation rdf:type :QuestionnaireValidationType;
    rdf:label "[object Object]".
:PreTest rdf:type :QuestionnaireValidationType;
    rdf:label "[object Object]".
:MathematicalValidation rdf:type :QuestionnaireValidationType;
    rdf:label "[object Object]".
:ConstructValidity rdf:type :QuestionnaireValidationType;
    rdf:label "[object Object]".
:CriterionValidity rdf:type :QuestionnaireValidationType;
    rdf:label "[object Object]".
:FaceValidity rdf:type :QuestionnaireValidationType;
    rdf:label "[object Object]".
:ReliabilityTesting rdf:type :QuestionnaireValidationType;
    rdf:label "[object Object]".
:CulturalValidation rdf:type :QuestionnaireValidationType;
    rdf:label "[object Object]".
:OtherValidation rdf:type :QuestionnaireValidationType;
    rdf:label "[object Object]".
:QuestionnaireValidationType rdfs:label "QuestionnaireValidationType"@en.
:QuestionnaireStatus rdf:type owl:Class, gufo:Kind, owl:NamedIndividual;
    rdfs:subClassOf gufo:IntrinsicMode;
    rdfs:label "QuestionnaireStatus"@en.
:QuestionnaireStatusType rdf:type owl:Class, gufo:AbstractIndividualType, owl:NamedIndividual;
    rdfs:subClassOf gufo:QualityValue;
    owl:equivalentClass [
  rdf:type owl:Class;
  owl:oneOf (:QuestionnaireDraft :QuestionnairePublished :QuestionnaireWithdrawn)
].
:QuestionnaireDraft rdf:type :QuestionnaireStatusType;
    rdf:label "[object Object]".
:QuestionnairePublished rdf:type :QuestionnaireStatusType;
    rdf:label "[object Object]".
:QuestionnaireWithdrawn rdf:type :QuestionnaireStatusType;
    rdf:label "[object Object]".
:QuestionnaireStatusType rdfs:label "QuestionnaireStatusType"@en.
:QuestionnaireLicence rdf:type owl:Class, gufo:Kind, owl:NamedIndividual;
    rdfs:subClassOf gufo:IntrinsicMode;
    rdfs:label "QuestionnaireLicence"@en.
:LicenceType rdf:type owl:Class, gufo:AbstractIndividualType, owl:NamedIndividual;
    rdfs:subClassOf gufo:QualityValue;
    owl:equivalentClass [
  rdf:type owl:Class;
  owl:oneOf (:Open :Proprietary :Hybrid :Other)
].
:Open rdf:type :LicenceType;
    rdf:label "[object Object]".
:Proprietary rdf:type :LicenceType;
    rdf:label "[object Object]".
:Hybrid rdf:type :LicenceType;
    rdf:label "[object Object]".
:Other rdf:type :LicenceType;
    rdf:label "[object Object]".
:LicenceType rdfs:label "LicenceType"@en.
:Author rdf:type owl:Class, gufo:Role, owl:NamedIndividual;
    rdfs:label "Author"@en.
:Authorship rdf:type owl:Class, gufo:Kind, owl:NamedIndividual;
    rdfs:subClassOf gufo:Relator;
    rdfs:label "Authorship"@en.
:Section rdf:type owl:Class, gufo:Kind, owl:NamedIndividual;
    rdfs:subClassOf gufo:VariableCollection;
    rdfs:label "Section"@en.
:Question rdf:type owl:Class, gufo:Kind, owl:NamedIndividual;
    rdfs:label "Question"@en.
:QuestionOrigin rdf:type owl:Class, gufo:Kind, owl:NamedIndividual;
    rdfs:subClassOf gufo:IntrinsicMode;
    rdfs:label "QuestionOrigin"@en.
:OpenQuestion rdf:type owl:Class, gufo:SubKind, owl:NamedIndividual;
    rdfs:label "OpenQuestion"@en.
:ClosedQuestion rdf:type owl:Class, gufo:SubKind, owl:NamedIndividual;
    rdfs:label "ClosedQuestion"@en.
:Variable rdf:type owl:Class, gufo:Kind, owl:NamedIndividual;
    rdfs:subClassOf gufo:FunctionalComplex;
    rdfs:label "Variable"@en.
:LatentVariable rdf:type owl:Class, gufo:SubKind, owl:NamedIndividual;
    rdfs:label "LatentVariable"@en.
:ObservableVariable rdf:type owl:Class, gufo:SubKind, owl:NamedIndividual;
    rdfs:label "ObservableVariable"@en.
:LevelsOfMeasurement rdf:type owl:Class, gufo:Kind, owl:NamedIndividual;
    rdfs:subClassOf gufo:IntrinsicMode;
    rdfs:label "LevelsOfMeasurement"@en.
:Scale rdf:type owl:Class, gufo:Kind, owl:NamedIndividual;
    rdfs:subClassOf gufo:IntrinsicMode;
    rdfs:label "Scale"@en.
:LevelsOfMeasurementType rdf:type owl:Class, gufo:AbstractIndividualType, owl:NamedIndividual;
    rdfs:subClassOf gufo:QualityValue;
    owl:equivalentClass [
  rdf:type owl:Class;
  owl:oneOf (:Nominal :Ordinal :Interval :Ratio)
].
:Nominal rdf:type :LevelsOfMeasurementType;
    rdf:label "[object Object]".
:Ordinal rdf:type :LevelsOfMeasurementType;
    rdf:label "[object Object]".
:Interval rdf:type :LevelsOfMeasurementType;
    rdf:label "[object Object]".
:Ratio rdf:type :LevelsOfMeasurementType;
    rdf:label "[object Object]".
:LevelsOfMeasurementType rdfs:label "LevelsOfMeasurementType"@en.
:ScaleType rdf:type owl:Class, gufo:AbstractIndividualType, owl:NamedIndividual;
    rdfs:subClassOf gufo:QualityValue;
    owl:equivalentClass [
  rdf:type owl:Class;
  owl:oneOf (:ChecklistScale :ComparativeScale :ConstantSumScale :DichotomousScale :ForcedRatingScale :GraphicRatingScale :GuttmanScale :IntervalQuestionScale :IpsativeScale :LikertScale :LikertTypeScale :MultipleChoiceScale :MultipleRatingListScale :NominalQuestionScale :PairedComparisonScale :SemanticDifferentialScale :SimpleCategoricalScale :StapelScale :ThurstoneScale :VisualAnalogScale)
].
:ChecklistScale rdf:type :ScaleType;
    rdf:label "[object Object]".
:ComparativeScale rdf:type :ScaleType;
    rdf:label "[object Object]".
:ConstantSumScale rdf:type :ScaleType;
    rdf:label "[object Object]".
:DichotomousScale rdf:type :ScaleType;
    rdf:label "[object Object]".
:ForcedRatingScale rdf:type :ScaleType;
    rdf:label "[object Object]".
:GraphicRatingScale rdf:type :ScaleType;
    rdf:label "[object Object]".
:GuttmanScale rdf:type :ScaleType;
    rdf:label "[object Object]".
:IntervalQuestionScale rdf:type :ScaleType;
    rdf:label "[object Object]".
:IpsativeScale rdf:type :ScaleType;
    rdf:label "[object Object]".
:LikertScale rdf:type :ScaleType;
    rdf:label "[object Object]".
:LikertTypeScale rdf:type :ScaleType;
    rdf:label "[object Object]".
:MultipleChoiceScale rdf:type :ScaleType;
    rdf:label "[object Object]".
:MultipleRatingListScale rdf:type :ScaleType;
    rdf:label "[object Object]".
:NominalQuestionScale rdf:type :ScaleType;
    rdf:label "[object Object]".
:PairedComparisonScale rdf:type :ScaleType;
    rdf:label "[object Object]".
:SemanticDifferentialScale rdf:type :ScaleType;
    rdf:label "[object Object]".
:SimpleCategoricalScale rdf:type :ScaleType;
    rdf:label "[object Object]".
:StapelScale rdf:type :ScaleType;
    rdf:label "[object Object]".
:ThurstoneScale rdf:type :ScaleType;
    rdf:label "[object Object]".
:VisualAnalogScale rdf:type :ScaleType;
    rdf:label "[object Object]".
:ScaleType rdfs:label "ScaleType"@en.
:ResponseOptions rdf:type owl:Class, gufo:Kind, owl:NamedIndividual;
    rdfs:subClassOf gufo:VariableCollection;
    rdfs:label "ResponseOptions"@en.
:ResponseOption rdf:type owl:Class, gufo:Kind, owl:NamedIndividual;
    rdfs:subClassOf gufo:FunctionalComplex;
    rdfs:label "ResponseOption"@en.
:QuestionOriginType rdf:type owl:Class, gufo:AbstractIndividualType, owl:NamedIndividual;
    rdfs:subClassOf gufo:QualityValue;
    owl:equivalentClass [
  rdf:type owl:Class;
  owl:oneOf (:Original :LiteralCopy :AdaptToContext :ReplaceTerms :Translation)
].
:Original rdf:type :QuestionOriginType;
    rdf:label "[object Object]".
:LiteralCopy rdf:type :QuestionOriginType;
    rdf:label "[object Object]".
:AdaptToContext rdf:type :QuestionOriginType;
    rdf:label "[object Object]".
:ReplaceTerms rdf:type :QuestionOriginType;
    rdf:label "[object Object]".
:Translation rdf:type :QuestionOriginType;
    rdf:label "[object Object]".
:QuestionOriginType rdfs:label "QuestionOriginType"@en.
:Ramification rdf:type owl:Class, gufo:SituationType, owl:NamedIndividual;
    rdfs:subClassOf gufo:Situation;
    rdfs:label "Ramification"@en.
:Questionnaire rdfs:subClassOf :DataCollectionInstrument.
:Author rdfs:subClassOf :Person.
:Question rdfs:subClassOf :Detector.
:OpenQuestion rdfs:subClassOf :Question.
:ClosedQuestion rdfs:subClassOf :Question.
:LatentVariable rdfs:subClassOf :Variable.
:ObservableVariable rdfs:subClassOf :Variable.
:hasName rdfs:domain :Person, :Questionnaire, :Section, :Question, :Variable;
    rdfs:range xsd:string;
    rdf:type owl:DatatypeProperty;
    rdfs:subPropertyOf gufo:hasQualityValue;
    rdfs:label "hasName"@en.
:hasUri rdfs:domain :Person, :Questionnaire, :QuestionnaireValidation, :QuestionnaireStatus, :QuestionnaireLicence, :Section, :Question, :Variable, :ResponseOption, :LevelsOfMeasurement, :Scale, :ResponseOptions;
    rdfs:range xsd:string;
    rdf:type owl:DatatypeProperty;
    rdfs:subPropertyOf gufo:hasQualityValue;
    rdfs:label "hasUri"@en.
:hasIdentifier rdfs:domain :Person, :Questionnaire, :QuestionnaireValidation, :QuestionnaireStatus, :QuestionnaireLicence, :Section, :Question, :Variable, :ResponseOption;
    rdfs:range xsd:string;
    rdf:type owl:DatatypeProperty;
    rdfs:subPropertyOf gufo:hasQualityValue;
    rdfs:label "hasIdentifier"@en.
:hasOrcid rdfs:domain :Person;
    rdfs:range xsd:string;
    rdf:type owl:DatatypeProperty;
    rdfs:subPropertyOf gufo:hasQualityValue;
    rdfs:label "hasOrcid"@en.
:hasLattes rdfs:domain :Person;
    rdfs:range xsd:string;
    rdf:type owl:DatatypeProperty;
    rdfs:subPropertyOf gufo:hasQualityValue;
    rdfs:label "hasLattes"@en.
:hasEmail rdfs:domain :Person;
    rdfs:range xsd:string;
    rdf:type owl:DatatypeProperty;
    rdfs:subPropertyOf gufo:hasQualityValue;
    rdfs:label "hasEmail"@en.
:hasFiliation rdfs:domain :Person;
    rdfs:range xsd:string;
    rdf:type owl:DatatypeProperty;
    rdfs:subPropertyOf gufo:hasQualityValue;
    rdfs:label "hasFiliation"@en.
:hasVersion rdfs:domain :Questionnaire;
    rdfs:range xsd:string;
    rdf:type owl:DatatypeProperty;
    rdfs:subPropertyOf gufo:hasQualityValue;
    rdfs:label "hasVersion"@en.
:hasDescription rdfs:domain :Questionnaire, :QuestionnaireValidation;
    rdfs:range xsd:string;
    rdf:type owl:DatatypeProperty;
    rdfs:subPropertyOf gufo:hasQualityValue;
    rdfs:label "hasDescription"@en.
:hasScoringInstructions rdfs:domain :Questionnaire;
    rdfs:range xsd:string;
    rdf:type owl:DatatypeProperty;
    rdfs:subPropertyOf gufo:hasQualityValue;
    rdfs:label "hasScoringInstructions"@en.
:hasBibliographicReference rdfs:domain :Questionnaire;
    rdfs:range xsd:string;
    rdf:type owl:DatatypeProperty;
    rdfs:subPropertyOf gufo:hasQualityValue;
    rdfs:label "hasBibliographicReference"@en.
:hasAcronym rdfs:domain :Questionnaire, :Section, :Question;
    rdfs:range xsd:string;
    rdf:type owl:DatatypeProperty;
    rdfs:subPropertyOf gufo:hasQualityValue;
    rdfs:label "hasAcronym"@en.
:hasMediaRepresentation rdfs:domain :Questionnaire;
    rdfs:range xsd:string;
    rdf:type owl:DatatypeProperty;
    rdfs:subPropertyOf gufo:hasQualityValue;
    rdfs:label "hasMediaRepresentation"@en.
:hasLanguage rdfs:domain :Questionnaire, :QuestionnaireValidation;
    rdfs:range xsd:string;
    rdf:type owl:DatatypeProperty;
    rdfs:subPropertyOf gufo:hasQualityValue;
    rdfs:label "hasLanguage"@en.
:hasPopulation rdfs:domain :QuestionnaireValidation;
    rdfs:range xsd:string;
    rdf:type owl:DatatypeProperty;
    rdfs:subPropertyOf gufo:hasQualityValue;
    rdfs:label "hasPopulation"@en.
:hasContext rdfs:domain :QuestionnaireValidation;
    rdfs:range xsd:string;
    rdf:type owl:DatatypeProperty;
    rdfs:subPropertyOf gufo:hasQualityValue;
    rdfs:label "hasContext"@en.
:hasMethodology rdfs:domain :QuestionnaireValidation;
    rdfs:range xsd:string;
    rdf:type owl:DatatypeProperty;
    rdfs:subPropertyOf gufo:hasQualityValue;
    rdfs:label "hasMethodology"@en.
:hasSampling rdfs:domain :QuestionnaireValidation;
    rdfs:range xsd:string;
    rdf:type owl:DatatypeProperty;
    rdfs:subPropertyOf gufo:hasQualityValue;
    rdfs:label "hasSampling"@en.
:hasLocation rdfs:domain :QuestionnaireValidation;
    rdfs:range xsd:string;
    rdf:type owl:DatatypeProperty;
    rdfs:subPropertyOf gufo:hasQualityValue;
    rdfs:label "hasLocation"@en.
:hasBibliographicReference rdfs:domain :QuestionnaireValidation;
    rdfs:range xsd:string;
    rdf:type owl:DatatypeProperty;
    rdfs:subPropertyOf gufo:hasQualityValue;
    rdfs:label "hasBibliographicReference"@en.
:hasQuestionnaireValidationType rdfs:domain :QuestionnaireValidation;
    rdfs:range :QuestionnaireValidationType;
    rdf:type owl:ObjectProperty;
    rdfs:subPropertyOf gufo:hasReifiedQualityValue;
    rdfs:label "hasQuestionnaireValidationType"@en.
:hasQuestionnaireStatusType rdfs:domain :QuestionnaireStatus;
    rdfs:range :QuestionnaireStatusType;
    rdf:type owl:ObjectProperty;
    rdfs:subPropertyOf gufo:hasReifiedQualityValue;
    rdfs:label "hasQuestionnaireStatusType"@en.
:hasLicenceName rdfs:domain :QuestionnaireLicence;
    rdfs:range xsd:string;
    rdf:type owl:DatatypeProperty;
    rdfs:subPropertyOf gufo:hasQualityValue;
    rdfs:label "hasLicenceName"@en.
:hasLicenceDescription rdfs:domain :QuestionnaireLicence;
    rdfs:range xsd:string;
    rdf:type owl:DatatypeProperty;
    rdfs:subPropertyOf gufo:hasQualityValue;
    rdfs:label "hasLicenceDescription"@en.
:hasOwnerName rdfs:domain :QuestionnaireLicence;
    rdfs:range xsd:string;
    rdf:type owl:DatatypeProperty;
    rdfs:subPropertyOf gufo:hasQualityValue;
    rdfs:label "hasOwnerName"@en.
:hasWebsite rdfs:domain :QuestionnaireLicence;
    rdfs:range xsd:string;
    rdf:type owl:DatatypeProperty;
    rdfs:subPropertyOf gufo:hasQualityValue;
    rdfs:label "hasWebsite"@en.
:hasLicenceType rdfs:domain :QuestionnaireLicence;
    rdfs:range :LicenceType;
    rdf:type owl:ObjectProperty;
    rdfs:subPropertyOf gufo:hasReifiedQualityValue;
    rdfs:label "hasLicenceType"@en.
:hasTitle rdfs:domain :Section;
    rdfs:range xsd:string;
    rdf:type owl:DatatypeProperty;
    rdfs:subPropertyOf gufo:hasQualityValue;
    rdfs:label "hasTitle"@en.
:hasInstructions rdfs:domain :Section;
    rdfs:range xsd:string;
    rdf:type owl:DatatypeProperty;
    rdfs:subPropertyOf gufo:hasQualityValue;
    rdfs:label "hasInstructions"@en.
:hasHypertext rdfs:domain :Section, :Question, :Variable, :ResponseOption;
    rdfs:range xsd:string;
    rdf:type owl:DatatypeProperty;
    rdfs:subPropertyOf gufo:hasQualityValue;
    rdfs:label "hasHypertext"@en.
:hasPrimming rdfs:domain :Section;
    rdfs:range xsd:string;
    rdf:type owl:DatatypeProperty;
    rdfs:subPropertyOf gufo:hasQualityValue;
    rdfs:label "hasPrimming"@en.
:hasRandomQuestions rdfs:domain :Section;
    rdfs:range xsd:boolean;
    rdf:type owl:DatatypeProperty;
    rdfs:subPropertyOf gufo:hasQualityValue;
    rdfs:label "hasRandomQuestions"@en.
:hasInitialStatement rdfs:domain :Question;
    rdfs:range xsd:string;
    rdf:type owl:DatatypeProperty;
    rdfs:subPropertyOf gufo:hasQualityValue;
    rdfs:label "hasInitialStatement"@en.
:hasText rdfs:domain :Question, :ResponseOption, :Variable;
    rdfs:range xsd:string;
    rdf:type owl:DatatypeProperty;
    rdfs:subPropertyOf gufo:hasQualityValue;
    rdfs:label "hasText"@en.
:hasMarkdowntext rdfs:domain :Question;
    rdfs:range xsd:boolean;
    rdf:type owl:DatatypeProperty;
    rdfs:subPropertyOf gufo:hasQualityValue;
    rdfs:label "hasMarkdowntext"@en.
:isSkippable rdfs:domain :Question;
    rdfs:range xsd:boolean;
    rdf:type owl:DatatypeProperty;
    rdfs:subPropertyOf gufo:hasQualityValue;
    rdfs:label "isSkippable"@en.
:hasExternalConceptURI rdfs:domain :Question, :ResponseOption;
    rdfs:range xsd:string;
    rdf:type owl:DatatypeProperty;
    rdfs:subPropertyOf gufo:hasQualityValue;
    rdfs:label "hasExternalConceptURI"@en.
:hasOrder rdfs:domain :Question;
    rdfs:range xsd:string;
    rdf:type owl:DatatypeProperty;
    rdfs:subPropertyOf gufo:hasQualityValue;
    rdfs:label "hasOrder"@en.
:hasOriginType rdfs:domain :QuestionOrigin;
    rdfs:range :QuestionOriginType;
    rdf:type owl:ObjectProperty;
    rdfs:subPropertyOf gufo:hasReifiedQualityValue;
    rdfs:label "hasOriginType"@en.
:hasExpectedFormat rdfs:domain :Variable;
    rdfs:range xsd:string;
    rdf:type owl:DatatypeProperty;
    rdfs:subPropertyOf gufo:hasQualityValue;
    rdfs:label "hasExpectedFormat"@en.
:hasMinimumValue rdfs:domain :Variable;
    rdfs:range xsd:string;
    rdf:type owl:DatatypeProperty;
    rdfs:subPropertyOf gufo:hasQualityValue;
    rdfs:label "hasMinimumValue"@en.
:hasMaximumValue rdfs:domain :Variable;
    rdfs:range xsd:string;
    rdf:type owl:DatatypeProperty;
    rdfs:subPropertyOf gufo:hasQualityValue;
    rdfs:label "hasMaximumValue"@en.
:hasUnit rdfs:domain :Variable;
    rdfs:range xsd:string;
    rdf:type owl:DatatypeProperty;
    rdfs:subPropertyOf gufo:hasQualityValue;
    rdfs:label "hasUnit"@en.
:hasMeasurementInstructions rdfs:domain :LatentVariable;
    rdfs:range xsd:string;
    rdf:type owl:DatatypeProperty;
    rdfs:subPropertyOf gufo:hasQualityValue;
    rdfs:label "hasMeasurementInstructions"@en.
:hasLevelsOfMeasurementType rdfs:domain :LevelsOfMeasurement;
    rdfs:range :LevelsOfMeasurementType;
    rdf:type owl:ObjectProperty;
    rdfs:subPropertyOf gufo:hasReifiedQualityValue;
    rdfs:label "hasLevelsOfMeasurementType"@en.
:hasScaleType rdfs:domain :Scale;
    rdfs:range :ScaleType;
    rdf:type owl:ObjectProperty;
    rdfs:subPropertyOf gufo:hasReifiedQualityValue;
    rdfs:label "hasScaleType"@en.
:hasRandomResponseOptions rdfs:domain :ResponseOptions;
    rdfs:range xsd:boolean;
    rdf:type owl:DatatypeProperty;
    rdfs:subPropertyOf gufo:hasQualityValue;
    rdfs:label "hasRandomResponseOptions"@en.
:hasValue rdfs:domain :ResponseOption;
    rdfs:range xsd:string;
    rdf:type owl:DatatypeProperty;
    rdfs:subPropertyOf gufo:hasQualityValue;
    rdfs:label "hasValue"@en.
:hasCondition rdfs:domain :Ramification;
    rdfs:range xsd:string;
    rdf:type owl:DatatypeProperty;
    rdfs:subPropertyOf gufo:hasQualityValue;
    rdfs:label "hasCondition"@en.
:questionnaireValidationInvolvedQuestionnaire rdf:type owl:ObjectProperty;
    rdfs:domain :QuestionnaireValidation;
    rdfs:range :Questionnaire;
    rdfs:label "questionnaireValidationInvolvedQuestionnaire"@en;
    rdfs:subPropertyOf gufo:participatedIn.
:questionnaireStatusInheresInQuestionnaire rdf:type owl:ObjectProperty;
    rdfs:domain :QuestionnaireStatus;
    rdfs:range :Questionnaire;
    rdfs:label "questionnaireStatusInheresInQuestionnaire"@en;
    rdfs:subPropertyOf gufo:inheresIn.
:characterizationQuestionnaireLicence rdf:type owl:ObjectProperty;
    rdfs:domain :QuestionnaireLicence;
    rdfs:range :Questionnaire;
    rdfs:label "characterizationQuestionnaireLicence"@en;
    rdfs:subPropertyOf gufo:inheresIn.
:authorshipMediatesQuestionnaire rdf:type owl:ObjectProperty;
    rdfs:domain :Authorship;
    rdfs:range :Questionnaire;
    rdfs:label "authorshipMediatesQuestionnaire"@en;
    rdfs:subPropertyOf gufo:mediates.
:authorshipMediatesAuthor rdf:type owl:ObjectProperty;
    rdfs:domain :Authorship;
    rdfs:range :Author;
    rdfs:label "authorshipMediatesAuthor"@en;
    rdfs:subPropertyOf gufo:mediates.
:sectionIsCollectionMemberOfQuestionnaire rdf:type owl:ObjectProperty;
    rdfs:domain :Section;
    rdfs:range :Questionnaire;
    rdfs:label "sectionIsCollectionMemberOfQuestionnaire"@en;
    rdfs:subPropertyOf gufo:isCollectionMemberOf.
:questionIsComponentOfSection rdf:type owl:ObjectProperty;
    rdfs:domain :Question;
    rdfs:range :Section;
    rdfs:label "questionIsComponentOfSection"@en;
    rdfs:subPropertyOf gufo:isComponentOf.
:questionOriginInheresInQuestion rdf:type owl:ObjectProperty;
    rdfs:domain :QuestionOrigin;
    rdfs:range :Question;
    rdfs:label "questionOriginInheresInQuestion"@en;
    rdfs:subPropertyOf gufo:inheresIn.
:historicalDependenceOfObservableVariables rdf:type owl:ObjectProperty;
    rdfs:domain :LatentVariable;
    rdfs:range :ObservableVariable;
    rdfs:label "historicalDependenceOfObservableVariables"@en;
    rdfs:subPropertyOf gufo:historicallyDependsOn.
:observableVariableIsComponentOfClosedQuestion rdf:type owl:ObjectProperty;
    rdfs:domain :ObservableVariable;
    rdfs:range :ClosedQuestion;
    rdfs:label "observableVariableIsComponentOfClosedQuestion"@en;
    rdfs:subPropertyOf gufo:isComponentOf.
:characterizationClosedQuestionLevelsofMeasurement rdf:type owl:ObjectProperty;
    rdfs:domain :LevelsOfMeasurement;
    rdfs:range :ClosedQuestion;
    rdfs:label "characterizationClosedQuestionLevelsofMeasurement"@en;
    rdfs:subPropertyOf gufo:inheresIn.
:characterizationClosedQuestionScale rdf:type owl:ObjectProperty;
    rdfs:domain :Scale;
    rdfs:range :ClosedQuestion;
    rdfs:label "characterizationClosedQuestionScale"@en;
    rdfs:subPropertyOf gufo:inheresIn.
:responseOptionsIsComponentOfClosedQuestion rdf:type owl:ObjectProperty;
    rdfs:domain :ResponseOptions;
    rdfs:range :ClosedQuestion;
    rdfs:label "responseOptionsIsComponentOfClosedQuestion"@en;
    rdfs:subPropertyOf gufo:isComponentOf.
:responseOptionIsCollectionMemberOfResponseOptions rdf:type owl:ObjectProperty;
    rdfs:domain :ResponseOption;
    rdfs:range :ResponseOptions;
    rdfs:label "responseOptionIsCollectionMemberOfResponseOptions"@en;
    rdfs:subPropertyOf gufo:isCollectionMemberOf.
:hasNextSection rdf:type owl:ObjectProperty;
    rdfs:domain :Section;
    rdfs:range :Section;
    rdfs:label "hasNextSection"@en.
:hasDerivedFromQuestion rdf:type owl:ObjectProperty;
    rdfs:domain :QuestionOrigin;
    rdfs:range :Question;
    rdfs:label "hasDerivedFromQuestion"@en.
:hasDerivedFromQuestionnaire rdf:type owl:ObjectProperty;
    rdfs:domain :Questionnaire;
    rdfs:range :Questionnaire;
    rdfs:label "hasDerivedFromQuestionnaire"@en.
:fromQuestion rdf:type owl:ObjectProperty;
    rdfs:domain :Ramification;
    rdfs:range :Question;
    rdfs:label "fromQuestion"@en.
:toQuestion rdf:type owl:ObjectProperty;
    rdfs:domain :Ramification;
    rdfs:range :Question;
    rdfs:label "toQuestion"@en.

:Author rdfs:comment "Person responsible for the intellectual creation or original conception of the structural elements of a research instrument."@en,
        "Pessoa responsável pela criação intelectual ou concepção original dos elementos estruturantes de um instrumento de pesquisa."@pt-br .

:Authorship rdfs:comment "Relational construct that mediates the link between a person and the authorship of a questionnaire, enabling attribution and provenance tracking."@en,
        "Construto relacional que media a ligação entre uma pessoa e a autoria de um questionário, permitindo a atribuição e o rastreamento da proveniência."@pt-br .

:ClosedQuestion rdfs:comment "Question that presents predefined response options, limiting the answer space to a structured set."@en,
        "Questão que apresenta opções de resposta predefinidas, restringindo o espaço de resposta a um conjunto estruturado."@pt-br .

:Detector rdfs:comment "category of devices that detects measurements (such as temperature or wind speed) or records information (such as responses to a questionnaire)"@en,
        "categoria de dispositivos que detectam medições (como temperatura ou velocidade do vento) ou registram informações (como respostas a um questionário)"@pt-br .

:DataCollectionInstrument rdfs:comment "Artifact used for the structured and systematic acquisition of information, including physical, elicitation, or computational tools."@en,
        "Artefato utilizado para a aquisição estruturada e sistemática de informações, incluindo instrumentos físicos, de elicitação ou computacionais."@pt-br .

:LevelsOfMeasurement rdfs:comment "Characterization of the nature and properties of variables in terms of measurement theory (nominal, ordinal, interval, ratio)."@en,
        "Caracterização da natureza e propriedades das variáveis com base na teoria da mensuração (nominal, ordinal, intervalar, razão)."@pt-br .

:LevelsOfMeasurementType rdfs:comment "Enumeration of measurement levels indicating variable characteristics and statistical properties."@en,
        "Enumeração dos níveis de medida que indicam características e propriedades estatísticas das variáveis."@pt-br .

:LicenceType rdfs:comment "Enumeration of licence modalities defining reuse permissions and restrictions of questionnaires."@en,
        "Enumeração das modalidades de licença que definem permissões e restrições de reutilização de questionários."@pt-br .

:OpenQuestion rdfs:comment "Question type that allows respondents to provide free-form, unrestricted textual answers."@en,
        "Tipo de questão que permite ao respondente fornecer respostas textuais livres e não restritas."@pt-br .

:OriginType rdfs:comment "Classification of how a question or questionnaire was derived, such as through translation, adaptation, or literal copying."@en,
        "Classificação de como uma questão ou questionário foi derivado, como por meio de tradução, adaptação ou cópia literal."@pt-br .

:Person rdfs:comment "Individual who may assume roles such as author or validator in the context of questionnaire design and use."@en,
        "Indivíduo que pode assumir papéis como autor ou validador no contexto da concepção e uso de questionários."@pt-br .

:Question rdfs:comment "Type of detector designed to capture specific information from respondents through structured statements, which can assume an open format (allowing free responses) or closed format (with predetermined response options) depending on the objective of data collection."@en,
        "Tipo de detector destinado a captar informações específicas de respondentes por meio de enunciados estruturados, podendo assumir formato aberto (permitindo respostas livres) ou fechado (com opções de resposta predeterminadas) conforme o objetivo da coleta de dados."@pt-br .

:Questionnaire rdfs:comment "Data collection instrument used to obtain information provided by respondents from their responses to the questionnaire."@en,
        "Instrumento de coleta de dados utilizado para obter informações fornecidas por respondentes a partir de suas respostas ao questionário."@pt-br .

:QuestionnaireLicence rdfs:comment "Mode that characterizes the licensing condition under which the questionnaire can be reused."@en,
        "Modo que caracteriza a condição de licenciamento sob a qual o questionário pode ser reutilizado."@pt-br .

:QuestionnaireStatus rdfs:comment "State representation of the questionnaire lifecycle, such as draft, published, or withdrawn."@en,
        "Representação do estado do ciclo de vida do questionário, como rascunho, publicado ou retirado."@pt-br .

:QuestionnaireStatusType rdfs:comment "Enumeration of possible lifecycle statuses of a questionnaire."@en,
        "Enumeração dos possíveis estados do ciclo de vida de um questionário."@pt-br .

:QuestionnaireValidation rdfs:comment "Process undertaken to assess whether a questionnaire measures what it is intended to measure."@en,
        "Processo realizado para avaliar se um questionário mede efetivamente o que se propõe a mensurar."@pt-br .

:QuestionnaireValidationType rdfs:comment "Enumeration of methodological strategies used to validate a questionnaire, such as content, construct, or criterion validity."@en,
        "Enumeração de estratégias metodológicas utilizadas para validar um questionário, como validade de conteúdo, de construto ou de critério."@pt-br .

:ResponseOption rdfs:comment "Predefined alternative provided in closed questions for the elicitation of specific information."@en,
        "Alternativa predefinida oferecida em questões fechadas para a elicitação de informações específicas."@pt-br .

:ResponseOptions rdfs:comment "Represents a structured collection of response option type entities, comprising the set of all predefined alternatives associated with a closed question instance"@en,
        "Representa uma coleção estruturada de entidades do tipo opção de resposta, compondo o conjunto de todas as alternativas predefinidas associadas a uma instância de questão fechada."@pt-br .

:Scale rdfs:comment "Systematic technique used to operationalize and standardize the collection of structured responses."@en,
        "Técnica sistemática utilizada para operacionalizar e padronizar a coleta de respostas estruturadas."@pt-br .

:ScaleType rdfs:comment "Enumeration of scale categories, such as Likert, Multiple Choice, and Guttman, that define the structure of response collection."@en,
        "Enumeração das categorias de escala, como Likert, Múltipla Escolha e Guttman, que definem a estrutura da coleta de respostas."@pt-br .

:Section rdfs:comment "Subset of questions within a questionnaire, organized according to thematic or conceptual criteria."@en,
        "Subconjunto de perguntas dentro de um questionário, organizado segundo critérios temáticos ou conceituais."@pt-br .

:Variable rdfs:comment "Measurable attribute represented by a question, capable of assuming different values based on respondent choices."@en,
        "Atributo mensurável representado por uma questão, capaz de assumir diferentes valores conforme as escolhas dos respondentes."@pt-br .

:LatentVariable rdfs:comment "Variable whose values ​​can be measured directly through the objective collection of empirical data, without the need for inference."@en,
        "Variável que representa construtos teóricos não observáveis diretamente, sendo inferidos indiretamente a partir de múltiplas variáveis observáveis associadas."@pt-br .

:ObservableVariable rdfs:comment "Variable that represents an observable construct, which is directly measured or observed."@en,
        "Variável que cujos valores podem ser mensurados diretamente por meio da coleta objetiva de dados empíricos, sem necessidade de inferência."@pt-br .


:QuestionOrigin rdfs:comment "Mode that characterizes the provenance of a question, specifying whether it was newly created or derived from another instrument through processes such as translation, adaptation, or direct copying."@en , "Modo que caracteriza a proveniência de uma questão, especificando se ela foi criada originalmente ou derivada de outro instrumento por meio de processos como tradução, adaptação ou cópia direta."@pt-br .

:Ramification rdfs:comment "Situation representing the logical flow between questions in a questionnaire, where the response to one question determines the navigation path to another question."@en, "Situação que representa o fluxo lógico entre questões de um questionário, em que a resposta a uma questão determina o direcionamento do respondente para outra questão."@pt-br .

:authorshipMediatesAuthor rdfs:comment "Establishes the link between an authorship relationship and the person responsible for the authorship of the questionnaire."@en,
                          "Estabelece a vinculação entre uma relação de autoria e a pessoa responsável pela autoria do questionário."@pt-br .

:authorshipMediatesQuestionnaire rdfs:comment "Links an authorship relationship to the corresponding questionnaire."@en,
                                 "vincula uma relação de autoria ao questionário correspondente."@pt-br .

:characterizationQuestionnaireLicence rdfs:comment "Relates a questionnaire to the license that regulates its use, distribution or sharing."@en,
                                      "Relaciona um questionário à licença que regulamenta seu uso, distribuição ou compartilhamento."@pt-br .

:characterizationClosedQuestionLevelsofMeasurement rdfs:comment "Relates a closed question to the corresponding measurement level."@en,
                                             "Relaciona uma questão fechada ao nível de medida correspondente."@pt-br .

:characterizationClosedQuestionScale rdfs:comment "Represents the association between a closed question and the scale used to measure the responses."@en,
                                        "Representa a associação entre uma questão fechada e a escala utilizada para mensurar as respostas."@pt-br .

:fromQuestion rdfs:comment "Indicates the question from which a branching condition originates."@en,
                           "Indica a questão a partir da qual se origina uma condição de ramificação."@pt-br .

:hasDerivedFromQuestion rdfs:comment "Links the origin of a question to the very question from which it was derived or adapted."@en,
                                     "Vincula a origem de uma questão à própria questão da qual ela foi derivada ou adaptada."@pt-br .

:hasDerivedFromQuestionnaire rdfs:comment "Connects a questionnaire to the original questionnaire from which it was derived."@en,
                                          "Conecta um questionário ao questionário original do qual foi derivado."@pt-br .

:hasLevelsOfMeasurementType rdfs:comment "Specifies the type of measurement level—nominal, ordinal, interval, or ratio—assigned to responses to a closed-ended question."@en,
                                         "Especifica o tipo de nível de medida — nominal, ordinal, intervalar ou de razão — atribuído às respostas de uma questão fechada."@pt-br .

:hasLicenceType rdfs:comment "Defines the type of licence that applies to a questionnaire."@en,
                             "Define o tipo de licença que se aplica a um questionário."@pt-br .

:hasOriginType rdfs:comment "Specifies the type of source linked to the origin of a question, indicating whether it is original, literal copy, adaptation to context, term substitution, or translation"@en,
                            "Especifica o tipo de origem vinculado à origem de uma questão, indicando se ela é original, cópia literal, adaptação ao contexto, substituição de termos ou tradução."@pt-br .

:hasQuestionnaireStatusType rdfs:comment "Defines the status of the questionnaire, classifying it as under development, published or withdrawn"@en,
                                       "Define o status do questionário, classificando-o como em elaboração, publicado ou retirado."@pt-br .

:hasQuestionnaireValidationType rdfs:comment "Defines the type of questionnaire validation, classifying it as content validation, semantic validation, pre-test, mathematical validation, construct validity, criterion validity, apparent validity, reliability test, cultural validation or other type of validation."@en,
                                             "Define o tipo de validação do questionário, classificando-o como validação de conteúdo, semântica, pré-teste, validação matemática, validade de construto, validade de critério, validade aparente, teste de confiabilidade, validação cultural ou outro tipo de validação."@pt-br .

:hasScaleType rdfs:comment "Defines the type of scale, classifying it as checklist, comparative, constant sum, dichotomous, forced evaluation, graphic, Guttman, interval question, ipsative, Likert, Likert type, multiple choice, multiple evaluation list, nominal, paired comparison, semantic differential, simple categorical, Stapel, Thurstone or visual analogue."@en,
                           "Define o tipo de escala, classificando-a como checklist, comparativa, soma constante, dicotômica, avaliação forçada, gráfica, Guttman, de questão intervalar, ipsativa, Likert, tipo Likert, múltipla escolha, lista de múltiplas avaliações, nominal, comparação pareada, diferencial semântico, categórica simples, Stapel, Thurstone ou visual analógica."@pt-br .

:historicalDependenceOfObservableVariables rdfs:comment "Expresses the historical dependence relationship between a latent variable and observable variables that operationalize it."@en,
                                          "Expressa a relação de dependência histórica entre uma variável latente e variáveis observáveis que a operacionalizam."@pt-br .

:questionnaireValidationInvolvedQuestionnaire rdfs:comment "Relates a validation process to the questionnaire that was evaluated."@en,
                                           "Relaciona um processo de validação ao questionário que foi avaliado."@pt-br .

:questionIsComponentOfSection rdfs:comment "Establishes that a question belongs to a specific section within a questionnaire."@en,
                                          "Estabelece que uma questão pertence a uma seção específica dentro de um questionário."@pt-br .

:questionOriginInheresInQuestion rdfs:comment "Characterizes the origin of a particular question in a questionnaire."@en,
                                     "Indica que uma determinada origem aplica-se a uma questão específica."@pt-br .

:questionnaireStatusInheresInQuestionnaire rdfs:comment "Characterizes the origin of a particular question in a questionnaire."@en,
                                           "Caracteriza a origem de uma determinada questão de um questionário"@pt-br .

:responseOptionIsCollectionMemberOfResponseOptions rdfs:comment "Indicates that an answer choice makes up the set of answer choices available for a question."@en,
                                                   "Indica que uma opção de resposta compõe o conjunto de opções de resposta disponíveis para uma questão"@pt-br .

:responseOptionsIsComponentOfClosedQuestion rdfs:comment "States that a set of response options is a component of a closed question."@en,
                                            "Indica que um conjunto de opções de resposta é componente de uma questão fechada."@pt-br .

:sectionIsCollectionMemberOfQuestionnaire rdfs:comment "Relates a section as a component of a questionnaire."@en,
                                          "Relaciona uma seção como componente de um questionário."@pt-br .

:toQuestion rdfs:comment "Establishes the link between a branch and the question to which the questionnaire flow should direct the respondent"@en,
                         "Estabelece a ligação entre uma ramificação e a questão para a qual o fluxo do questionário deve direcionar o respondente."@pt-br .

:observableVariableIsComponentOfClosedQuestion rdfs:comment "It establishes the composition relationship in which an observable variable is part of a closed question in the questionnaire."@en,
                                      "Estabelece a relação de composição em que uma variável observável integra uma questão fechada do questionário."@pt-br .

:hasAcronym rdfs:comment "Indicates the acronym of a questionnaire or its components."@en,
                         "Indica a sigla de um questionário ou de seus componentes."@pt-br .


:hasBibliographicReference rdfs:comment "Specifies the bibliographic reference supporting the questionnaire or its components."@en,
                           "Especifica a referência bibliográfica que fundamenta o questionário ou seus componentes."@pt-br .

:hasCondition rdfs:comment "Indicates a logical condition that must be satisfied for an action or question to be activated."@en,
                          "Indica uma condição lógica que deve ser satisfeita para que uma ação ou questão seja ativada."@pt-br .

:hasContext rdfs:comment "Defines the contextual domain in which a questionnaire or question is applicable."@en,
                         "Define o domínio contextual em que um questionário ou questão é aplicável."@pt-br .

:hasExternalConceptURI rdfs:comment "Indicates the URL that references an external class or concept that semantically describes the question or response option of the questionnaire."@en,
                                 "Indica a URL que referencia uma classe ou conceito externo que descreve semanticamente a questão ou opção de resposta do questionário."@pt-br .

:hasDescription rdfs:comment "Provides a textual description of the entity's content or purpose."@en,
                            "Fornece uma descrição textual sobre o conteúdo ou propósito da entidade."@pt-br .

:hasEmail rdfs:comment "Indicates the email address associated with a person or responsible entity."@en,
                       "Indica o endereço de e-mail associado a uma pessoa ou entidade responsável."@pt-br .

:hasEndPointInXSDDdate rdfs:comment "Represents the end date of a period associated with the entity."@en,
                                 "Representa a data de término de um período associado à entidade."@pt-br .

:hasExpectedFormat rdfs:comment "Indicates the expected data format for the response to a question."@en,
                              "Indica o formato de dado esperado para a resposta a uma questão."@pt-br .

:hasFiliation rdfs:comment "Links a person to their institutional affiliation."@en,
                          "Relaciona uma pessoa à sua afiliação institucional."@pt-br .

:hasHypertext rdfs:comment "Associates a hypertext link or content for reference or navigation."@en,
                          "Associa um link ou conteúdo em hipertexto para referência ou navegação."@pt-br .

:hasIdentifier rdfs:comment "Provides a unique identifier for the entity."@en,
                            "Fornece um identificador único para a entidade."@pt-br .

:hasInitialStatement rdfs:comment "Specifies an introductory text presented before a question to provide context or instruction."@en,
                                  "Especifica um texto introdutório apresentado antes de uma questão para fornecer contexto ou instruções."@pt-br .

:hasInstructions rdfs:comment "Defines instructions for answering a question or completing a questionnaire."@en,
                             "Define instruções para responder a uma questão ou completar um questionário."@pt-br .

:hasLanguage rdfs:comment "Indicates the language in which a question or questionnaire is expressed."@en,
                          "Indica o idioma no qual uma questão ou questionário está expressa."@pt-br .

:hasLattes rdfs:comment "Links a person to their Lattes CV identifier in the Brazilian academic system."@en,
                        "Relaciona uma pessoa ao identificador de seu currículo Lattes no sistema acadêmico brasileiro."@pt-br .

:hasLicenceDescription rdfs:comment "Provides a detailed textual description of the usage licence."@en,
                                   "Fornece uma descrição textual detalhada da licença de uso."@pt-br .

:hasLicenceName rdfs:comment "Indicates the name of the licence associated with a questionnaire."@en,
                             "Indica o nome da licença associada a um questionário."@pt-br .

:hasLocation rdfs:comment "Specifies the location relevant to the questionnaire or its application."@en,
                         "Especifica a localização relevante ao questionário ou sua aplicação."@pt-br .

:hasMarkdowntext rdfs:comment "Contains text formatted using Markdown for improved visualization."@en,
                              "Contém texto formatado em Markdown para melhor visualização."@pt-br .

:hasMaximumValue rdfs:comment "Specifies the upper bound of values allowed for a quantitative response."@en,
                              "Especifica o limite superior de valores permitidos para uma resposta quantitativa."@pt-br .

:hasMediaRepresentation rdfs:comment "Associates a media representation such as image, audio, or video with a question or questionnaire."@en,
                                     "Associa uma representação midiática como imagem, áudio ou vídeo a uma questão ou questionário."@pt-br .

:hasMethodology rdfs:comment "Describes the methodological basis underlying the questionnaire or its validation."@en,
                             "Descreve a base metodológica subjacente ao questionário ou à sua validação."@pt-br .

:hasMinimumValue rdfs:comment "Specifies the lower bound of values allowed for a quantitative response."@en,
                              "Especifica o limite inferior de valores permitidos para uma resposta quantitativa."@pt-br .

:hasName rdfs:comment "Denotes the full name of an entity, such as a person, questionnaire, or organization."@en,
                      "Denota o nome completo de uma entidade, como uma pessoa, questionário ou organização."@pt-br .

:hasOrcid rdfs:comment "Specifies the ORCID identifier associated with a researcher."@en,
                       "Especifica o identificador ORCID associado a um pesquisador."@pt-br .

:hasOrder rdfs:comment "Indicates the sequential order of presentation or application of an item."@en,
                       "Indica a ordem sequencial de apresentação ou aplicação de um item."@pt-br .

:hasOwner rdfs:comment "Relates an entity to the organization or individual responsible for its maintenance or authorship."@en,
                       "Relaciona uma entidade à organização ou indivíduo responsável por sua manutenção ou autoria."@pt-br .

:hasPopulation rdfs:comment "Specifies the population or group targeted by the questionnaire."@en,
                            "Especifica a população ou grupo-alvo do questionário."@pt-br .

:hasPrimming rdfs:comment "Indicates the priming text or stimulus preceding a question to influence interpretation or attention."@en,
                          "Indica o texto ou estímulo de preparação que antecede uma questão para influenciar sua interpretação ou atenção."@pt-br .

:hasRandomQuestions rdfs:comment "Indicates whether the questions in the questionnaire are randomly ordered."@en,
                          "Indica se as questões do questionário estão ordenadas aleatoriamente."@pt-br .

:hasRandomResponseOptions rdfs:comment "Indicates whether the answer options for a given question are randomly ordered."@en,
                          "Indica se as opções de resposta de uma determinada questão estão ordenadas aleatoriamente."@pt-br .

:hasSampling rdfs:comment "Describes the sampling method used in the research study associated with the questionnaire."@en,
                          "Descreve o método de amostragem utilizado no estudo de pesquisa associado ao questionário."@pt-br .

:hasScoringInstructions rdfs:comment "Provides instructions on how to score or interpret responses to a questionnaire."@en,
                                    "Fornece instruções sobre como pontuar ou interpretar as respostas de um questionário."@pt-br .

:hasText rdfs:comment "Contains the literal text of a question, answer option, or section title."@en,
                      "Contém o texto literal de uma questão, opção de resposta ou título de seção."@pt-br .

:hasTitle rdfs:comment "Indicates the formal title of the questionnaire or any of its parts."@en,
                       "Indica o título formal do questionário ou de qualquer uma de suas partes."@pt-br .

:hasUnit rdfs:comment "Denotes the unit of measurement expected for responses to a question."@en,
                      "Denota a unidade de medida esperada para as respostas de uma questão."@pt-br .

:hasUri rdfs:comment "Specifies a Uniform Resource Identifier (URI) that uniquely identifies the resource."@en,
                     "Especifica um Identificador Uniforme de Recurso (URI) que identifica unicamente o recurso."@pt-br .

:hasValue rdfs:comment "Holds the literal or numerical value assigned to a property or variable."@en,
                       "Contém o valor literal ou numérico atribuído a uma propriedade ou variável."@pt-br .

:hasVersion rdfs:comment "Indicates the version number or label of a questionnaire or element."@en,
                         "Indica o número ou rótulo de versão de um questionário ou elemento."@pt-br .

:hasWebsite rdfs:comment "Provides a URL that links to the official website of a questionnaire or its authors."@en,
                         "Fornece uma URL que remete ao site oficial de um questionário ou de seus autores."@pt-br .

:isSkippable rdfs:comment "Indicates whether a question can be optionally skipped by the respondent."@en,
                          "Indica se uma questão pode ser opcionalmente pulada pelo respondente."@pt-br .
